First proof for isin

BTree.thy
@@ -4,6 +4,7 @@ begin
 
 text "General structure:  nat values in the leafs and nat/tree node internal node list (nat always larger than every element in the corresponding subtree)"
 (* definition heavily based on Tree234_Set, Pair structure from ...*)
+(* TODO should all basic definitions be more abstract and use later refinements for implementations *)
 
 datatype btree = Leaf | Node "(btree * nat) list"
 
@@ -35,12 +36,21 @@ lemma set_eq_fold:"Suc (fold max xs 0) = Suc (Max (set (0#xs)))"
 value "(Node [(Leaf, 1), (Node [(Leaf, 1), (Leaf, 10)], 10), (Leaf, 30), (Leaf, 100)])"
 value "inorder (Node [(Leaf, 1), (Node [(Leaf, 1), (Leaf, 10)], 10), (Leaf, 30), (Leaf, 100)])"
 
-fun children where
-"children Leaf = {}" |
-"children (Node xs) = (set (map fst xs))"
+fun subtrees where "subtrees xs = (map fst xs)"
+fun seperators where "seperators xs = (map fst xs)"
 
 definition btree_set:: "btree \<Rightarrow> nat set" where 
   "btree_set = set \<circ> inorder"
+
+fun btree_set_alt:: "btree \<Rightarrow> nat set" where
+"btree_set_alt Leaf = {}" |
+"btree_set_alt (Node t) = set (map snd t) \<union> \<Union> (set (map (btree_set_alt) (subtrees t)))"
+
+
+fun bal:: "btree \<Rightarrow> bool" where
+"bal Leaf = True" |
+"bal (Node t) = ((\<forall>sub \<in> set (subtrees t). bal sub) \<and> (\<exists>h.\<forall>sub \<in> set (subtrees t). h = height sub))"
+
 
 fun btree_list:: "(btree * nat) list \<Rightarrow> bool" where
  "btree_list [] = True" |
@@ -72,6 +82,7 @@ lemma [simp]: "btree_list_choose y t = Subtree x2 \<Longrightarrow>
   apply (metis (no_types, lifting) dual_order.strict_trans less_Suc_eq less_add_Suc1 list_result.distinct(5) list_result.inject not_add_less2 not_less_eq)
   done
 
+
 fun isin where
  "isin y (Leaf) = False" |
  "isin y (Node t) = (case btree_list_choose y t of Nomatch \<Rightarrow> False | Match \<Rightarrow> True | Subtree sub \<Rightarrow> isin y sub)"
@@ -87,6 +98,11 @@ lemma append_foldr_set: "set (foldr (@) xs []) = \<Union> (set (map set xs))"
   apply(induction xs)
    apply(auto)
   done
+
+lemma btree_set_set_def: "btree_set t = btree_set_alt t"
+  apply(induction t)
+   apply(auto simp add: btree_set_def append_foldr_set)
+  by (metis image_eqI snd_conv)
 
 lemma child_subset: "p \<in> set t \<Longrightarrow> btree_set (fst p) \<subseteq> btree_set (Node t)"
   apply(induction p arbitrary: t)
@@ -104,14 +120,27 @@ lemma some_child_match: "btree_list_choose y t = Match \<Longrightarrow> y \<in>
    apply(auto simp add: cmp_def)
   by (metis list_result.distinct(6))
 
-lemma "isin y t = True \<Longrightarrow> y \<in> btree_set t"
-proof(induction y t rule: isin.induct)
-  case (1 y)
-  then show ?case by simp
-next
+lemma isin_true_not_nomatch: "isin y (Node t) = True \<Longrightarrow> btree_list_choose y t \<noteq> Nomatch"
+  by auto
+
+
+lemma "isin y n = True \<Longrightarrow> y \<in> btree_set n"
+proof(induction y n rule: isin.induct)
   case (2 y t)
-then show ?case sorry
-qed
+  then have "btree_list_choose y t = Match \<or> (\<exists>sub. btree_list_choose y t = Subtree sub)"
+    using isin_true_not_nomatch list_result.exhaust by blast
+  then show ?case
+  proof
+    assume "btree_list_choose y t = Match"
+    then show "y \<in> btree_set (Node t)" using some_child_match btree_set_set_def by auto
+  next
+    assume "\<exists>sub. btree_list_choose y t = Subtree sub"
+    then obtain sub where "btree_list_choose y t = Subtree sub" by blast
+    then show "y \<in> btree_set (Node t)"   
+      using some_child_sub btree_set_set_def 2 by force
+  qed
+qed simp
+
 
 
 end
